Cubical: missed a rename; SubLayer

theories/Cubical/Cubical.v
@@ -14,16 +14,16 @@ Set Keyed Unification.
 Remove Printing Let sigT.
 Remove Printing Let prod.
 
-Universe l'.
-Universe l.
+Universe m'.
+Universe m.
 
 Parameter side: HSet.
 
 (* PartialFrame consists of an 0-cells, and fillers which are the 1-cells,
    2-cells, and 3-cells relating the different 0-cells on the filler. *)
-Class PartialFramePrev (n: nat) (csp: Type@{l'}) := { (* csp: CubeSetPrefix *)
-  frame' {p} (Hp: p.+1 <= n): csp -> HSet@{l};
-  frame'' {p} (Hp: p.+2 <= n): csp -> HSet@{l};
+Class PartialFramePrev (n: nat) (csp: Type@{m'}) := { (* csp: CubeSetPrefix *)
+  frame' {p} (Hp: p.+1 <= n): csp -> HSet@{m};
+  frame'' {p} (Hp: p.+2 <= n): csp -> HSet@{m};
   restrFrame' {p q} {Hpq: p.+2 <= q.+2} (Hq: q.+2 <= n) (ε: side) {D: csp}:
     frame' (↓ (Hpq ↕ Hq)) D -> frame'' (Hpq ↕ Hq) D;
 }.
@@ -32,9 +32,9 @@ Arguments frame' {n csp} _ {p} Hp D.
 Arguments frame'' {n csp} _ {p} Hp D.
 Arguments restrFrame' {n csp} _ {p q Hpq} Hq ε {D} d.
 
-Class PartialFrame (n p: nat) (csp: Type@{l'})
+Class PartialFrame (n p: nat) (csp: Type@{m'})
   (FramePrev: PartialFramePrev n csp) := {
-  frame (Hp: p <= n): csp -> HSet@{l};
+  frame (Hp: p <= n): csp -> HSet@{m};
   restrFrame {q} {Hpq: p.+1 <= q.+1} (Hq: q.+1 <= n) (ε: side) {D: csp}:
     frame (↓ (Hpq ↕ Hq)) D -> FramePrev.(frame') (Hpq ↕ Hq) D;
   cohFrame {q r} {Hpr: p.+2 <= r.+2} {Hrq: r.+2 <= q.+2} {Hq: q.+2 <= n}
@@ -54,10 +54,10 @@ Arguments cohFrame {n p csp FramePrev} _ {q r Hpr Hrq Hq ε ω D} d.
 (* We build fillers using an iterated construction: a filler at level n depends
    on cubes at level n-1 and n-2; just as we have frame' and frame'', we have
    filler' and filler''. *)
-Class PartialFillerPrev (n: nat) (csp: Type@{l'})
+Class PartialFillerPrev (n: nat) (csp: Type@{m'})
   (FramePrev : PartialFramePrev n (@csp)) := {
-  filler' {p} {Hp: p.+1 <= n} {D: csp}: FramePrev.(frame') Hp D -> HSet@{l};
-  filler'' {p} {Hp: p.+2 <= n} {D: csp}: FramePrev.(frame'') Hp D -> HSet@{l};
+  filler' {p} {Hp: p.+1 <= n} {D: csp}: FramePrev.(frame') Hp D -> HSet@{m};
+  filler'' {p} {Hp: p.+2 <= n} {D: csp}: FramePrev.(frame'') Hp D -> HSet@{m};
   restrFiller' {p q} {Hpq: p.+2 <= q.+2} (Hq: q.+2 <= n) (ε: side) {D: csp}
     {d : FramePrev.(frame') (↓ (Hpq ↕ Hq)) D}:
     filler' d -> filler'' (FramePrev.(restrFrame') Hq ε d);
@@ -67,20 +67,20 @@ Arguments filler' {n csp FramePrev} _ {p Hp D} d.
 Arguments filler'' {n csp FramePrev} _ {p Hp D} d.
 Arguments restrFiller' {n csp FramePrev} _ {p q Hpq} Hq ε {D} [d] b.
 
-(* Cube consists of filler, restrFiller, and coherence conditions between them *)
-Class PartialFiller (n: nat) (csp: Type@{l'})
+(* Filler consists of filler, restrFiller, and coherence conditions between them *)
+Class PartialFiller (n: nat) (csp: Type@{m'})
   {FramePrev: PartialFramePrev n (@csp)}
   (FillerPrev: PartialFillerPrev n csp FramePrev)
   (Frame: forall {p}, PartialFrame n p (@csp) FramePrev) := {
   filler {p} {Hp: p <= n} {D: csp}:
-    (Frame.(frame) (¹ n) D -> HSet@{l}) -> Frame.(frame) Hp D -> HSet@{l};
+    (Frame.(frame) (¹ n) D -> HSet@{m}) -> Frame.(frame) Hp D -> HSet@{m};
   restrFiller {p q} {Hpq: p.+1 <= q.+1}
-    (Hq: q.+1 <= n) (ε: side) {D : csp} {E : Frame.(frame) (¹ n) D -> HSet@{l}}
+    (Hq: q.+1 <= n) (ε: side) {D : csp} {E : Frame.(frame) (¹ n) D -> HSet@{m}}
     {d : Frame.(frame) (↓ (Hpq ↕ Hq)) D} (c : filler E d):
     FillerPrev.(filler') (Frame.(restrFrame) Hq ε d);
   cohFiller {p q r} {Hpr: p.+2 <= r.+2}
     {Hrq: r.+2 <= q.+2} {Hq: q.+2 <= n}
-    (ε: side) (ω : side) {D: csp} (E: Frame.(frame) (¹ n) D -> HSet@{l})
+    (ε: side) (ω : side) {D: csp} (E: Frame.(frame) (¹ n) D -> HSet@{m})
     (d: Frame.(frame) (↓ (⇓ Hpr ↕ (↓ (Hrq ↕ Hq)))) D) (c: filler E d):
     rew [FillerPrev.(filler'')] (Frame.(cohFrame) d) in
     FillerPrev.(restrFiller') (Hpq := Hpr ↕ Hrq) Hq
@@ -93,22 +93,22 @@ Arguments filler {n csp FramePrev FillerPrev Frame} _ {p Hp D} E.
 Arguments restrFiller {n csp FramePrev FillerPrev Frame} _ {p q Hpq Hq ε D E} [d] c.
 Arguments cohFiller {n csp FramePrev FillerPrev Frame} _ {p q r Hpr Hrq Hq ε ω D E d} c.
 
-(* Cube consists of CubeSetPrefix, a box built out of partial boxes,
+(* Filler consists of CubeSetPrefix, a box built out of partial boxes,
   a filler built out of partial cubes, and some axioms related to our
   construction. *)
-Class Cubical (n : nat) := {
-  csp: Type@{l'};
+Class NType (n : nat) := {
+  csp: Type@{m'};
   FramePrev: PartialFramePrev n csp;
   Frame {p}: PartialFrame n p csp FramePrev;
   FillerPrev: PartialFillerPrev n csp FramePrev;
-  Cube: PartialFiller n csp FillerPrev (@Frame);
+  Filler: PartialFiller n csp FillerPrev (@Frame);
 
   (* Abbreviations corresponding to coherence conditions in Box *)
   Layer' {p} {Hp: p.+1 <= n} {D: csp} (d: Frame.(frame) (↓ Hp) D) :=
     hforall ε, FillerPrev.(filler') (Frame.(restrFrame) Hp ε d);
   Layer'' {p} {Hp: p.+2 <= n} {D: csp} (d: FramePrev.(frame') (↓ Hp) D) :=
     hforall ε, FillerPrev.(filler'') (FramePrev.(restrFrame') Hp ε d);
-  SubLayer' {p q ε} {Hpq: p.+2 <= q.+2} {Hq: q.+2 <= n} {D: csp}
+  RestrLayer' {p q ε} {Hpq: p.+2 <= q.+2} {Hq: q.+2 <= n} {D: csp}
     (d: Frame.(frame) (↓ ↓ (Hpq ↕ Hq)) D) (l: Layer' d):
       Layer'' (Frame.(restrFrame) Hq ε d) :=
   fun ω => rew [FillerPrev.(filler'')] Frame.(cohFrame) (Hrq := Hpq) d in FillerPrev.(restrFiller') Hq ε (l ω);
@@ -119,7 +119,8 @@ Class Cubical (n : nat) := {
   eqFrameSp {p} {Hp: p.+1 <= n} {D: csp}:
     Frame.(frame) Hp D = {d: Frame.(frame) (↓ Hp) D & Layer' d} :> Type;
   eqFrameSp' {p} {Hp: p.+2 <= n} {D: csp}:
-    FramePrev.(frame') Hp D = {d : FramePrev.(frame') (↓ Hp) D & Layer'' d} :> Type;
+    FramePrev.(frame') Hp D = {d : FramePrev.(frame') (↓ Hp) D & Layer'' d}
+      :> Type;
   eqRestrFrame0 {q} {Hpq: 1 <= q.+1} {Hq: q.+1 <= n} {ε: side} {D: csp}:
     Frame.(restrFrame) (Hpq := Hpq) Hq ε (rew <- [id] eqFrame0 (D := D) in tt) =
       (rew <- [id] eqFrame0' in tt);
@@ -127,31 +128,32 @@ Class Cubical (n : nat) := {
     {d: Frame.(frame) (↓ ↓ (Hpq ↕ Hq)) D}
     {l: Layer' (Hp := ↓ (Hpq ↕ Hq)) d}:
     Frame.(restrFrame) Hq ε (rew <- [id] eqFrameSp in (d; l)) =
-      rew <- [id] eqFrameSp' in (Frame.(restrFrame) Hq ε d; SubLayer' d l);
+      rew <- [id] eqFrameSp' in (Frame.(restrFrame) Hq ε d; RestrLayer' d l);
   eqFillerSp {p} {Hp: p.+1 <= n} {D: csp} {E d}:
-    Cube.(filler) (Hp := ↓ Hp) E d = {l: Layer' d &
-      Cube.(filler) (D := D) E (rew <- [id] eqFrameSp in (d; l))} :> Type;
+    Filler.(filler) (Hp := ↓ Hp) E d = {l: Layer' d &
+      Filler.(filler) (D := D) E (rew <- [id] eqFrameSp in (d; l))} :> Type;
   eqFillerSp' {p} {Hp: p.+2 <= n} {D: csp} {d}:
     FillerPrev.(filler') (Hp := ↓ Hp) d = {b : Layer'' d &
       FillerPrev.(filler') (rew <- [id] eqFrameSp' (D := D) in (d; b))} :> Type;
   eqRestrFiller0 {p} {Hp: p.+1 <= n} {D: csp} {E} {d} {ε: side}
-    {l: Layer' d} {Q: Cube.(filler) (D := D) E (rew <- eqFrameSp in (d; l))}:
-      l ε = Cube.(restrFiller) (Hq := Hp) (rew <- [id] eqFillerSp in (l; Q));
+    {l: Layer' d} {Q: Filler.(filler) (D := D) E (rew <- eqFrameSp in (d; l))}:
+      l ε = Filler.(restrFiller) (Hq := Hp) (rew <- [id] eqFillerSp in (l; Q));
   eqRestrFillerSp {p q} {Hpq: p.+2 <= q.+2} {Hq: q.+2 <= n} {D: csp} {E} {d}
     {ε: side} {l: Layer' (Hp := ↓ (Hpq ↕ Hq)) d}
-    {Q: Cube.(filler) (D := D) E (rew <- eqFrameSp in (d; l))}:
-    Cube.(restrFiller) (Hpq := ↓ Hpq) (ε := ε) (rew <- [id] eqFillerSp in (l; Q)) = rew <- [id] eqFillerSp' (Hp := Hpq ↕ Hq) in
-      (SubLayer' d l; rew [FillerPrev.(filler')] eqRestrFrameSp in Cube.(restrFiller) Q);
+    {Q: Filler.(filler) (D := D) E (rew <- eqFrameSp in (d; l))}:
+    Filler.(restrFiller) (Hpq := ↓ Hpq) (ε := ε) (rew <- [id] eqFillerSp in (l; Q)) = rew <- [id] eqFillerSp' (Hp := Hpq ↕ Hq) in
+      (RestrLayer' d l; rew [FillerPrev.(filler')] eqRestrFrameSp in
+        Filler.(restrFiller) Q);
 }.
 
 Arguments csp {n} _.
 Arguments FramePrev {n} _.
 Arguments FillerPrev {n} _.
 Arguments Frame {n} _ {p}.
-Arguments Cube {n} _.
+Arguments Filler {n} _.
 Arguments Layer' {n} _ {p Hp D} d.
 Arguments Layer'' {n} _ {p Hp D} d.
-Arguments SubLayer' {n} _ {p q} ε {Hpq Hq D d} l.
+Arguments RestrLayer' {n} _ {p q} ε {Hpq Hq D d} l.
 Arguments eqFrame0 {n} _ {len0 D}.
 Arguments eqFrame0' {n} _ {len1 D}.
 Arguments eqFrameSp {n} _ {p Hp D}.
@@ -164,11 +166,11 @@ Arguments eqRestrFiller0 {n} _ {p Hp D E d ε l Q}.
 Arguments eqRestrFillerSp {n} _ {p q Hpq Hq D E d ε l Q}.
 
 (* The csp at universe l' *)
-Definition mkcsp {n} {C: Cubical n}: Type@{l'} :=
-  sigT (fun D : C.(csp) => C.(Frame).(frame) (¹ n) D -> HSet@{l}).
+Definition mkcsp {n} {C: NType n}: Type@{m'} :=
+  sigT (fun D : C.(csp) => C.(Frame).(frame) (¹ n) D -> HSet@{m}).
 
 (* The previous level of Box *)
-Definition mkFramePrev {n} {C: Cubical n}: PartialFramePrev n.+1 mkcsp := {|
+Definition mkFramePrev {n} {C: NType n}: PartialFramePrev n.+1 mkcsp := {|
   frame' (p: nat) (Hp: p.+1 <= n.+1) (D: mkcsp) := C.(Frame).(frame) (⇓ Hp) D.1;
   frame'' (p: nat) (Hp: p.+2 <= n.+1) (D: mkcsp) :=
     C.(FramePrev).(frame') (⇓ Hp) D.1;
@@ -180,19 +182,19 @@ Definition mkFramePrev {n} {C: Cubical n}: PartialFramePrev n.+1 mkcsp := {|
 (* The coherence conditions that Box needs to satisfy to build the next level
    of Frame. These will be used in the proof script of mkFrame. *)
 
-Definition mkLayer {n p} {Hp: p.+1 <= n.+1} {C: Cubical n} {D: mkcsp}
+Definition mkLayer {n p} {Hp: p.+1 <= n.+1} {C: NType n} {D: mkcsp}
   {Frame: PartialFrame n.+1 p mkcsp mkFramePrev} {d: Frame.(frame) (↓ Hp) D}: HSet :=
-  hforall ε, C.(Cube).(filler) D.2 (Frame.(restrFrame) (Hpq := ¹ _) Hp ε d).
+  hforall ε, C.(Filler).(filler) D.2 (Frame.(restrFrame) (Hpq := ¹ _) Hp ε d).
 
-Definition mkSubLayer {n p q} {ε: side} {Hpq: p.+2 <= q.+2} {Hq: q.+2 <= n.+1}
-  {C: Cubical n} {D: mkcsp} {Frame: PartialFrame n.+1 p mkcsp mkFramePrev}
+Definition mkRestrLayer {n p q} {ε: side} {Hpq: p.+2 <= q.+2} {Hq: q.+2 <= n.+1}
+  {C: NType n} {D: mkcsp} {Frame: PartialFrame n.+1 p mkcsp mkFramePrev}
   (d: Frame.(frame) (↓ ↓ (Hpq ↕ Hq)) D)
   (l: mkLayer): C.(Layer') (Frame.(restrFrame) Hq ε d) :=
   fun ω => rew [C.(FillerPrev).(filler')] Frame.(cohFrame) d in
-    C.(Cube).(restrFiller) (Hpq := ⇓ Hpq) (l ω).
+    C.(Filler).(restrFiller) (Hpq := ⇓ Hpq) (l ω).
 
 Definition cohFrameSnHyp {n p q r} {ε ω: side} {Hpr: p.+3 <= r.+3}
-  {Hrq: r.+3 <= q.+3} {Hq: q.+3 <= n.+1} {C: Cubical n} {D: mkcsp}
+  {Hrq: r.+3 <= q.+3} {Hq: q.+3 <= n.+1} {C: NType n} {D: mkcsp}
   {frame': PartialFrame n.+1 p mkcsp mkFramePrev}
   {d: frame'.(frame) (↓ ↓ ↓ (Hpr ↕ Hrq ↕ Hq)) D}:
   C.(Frame).(restrFrame) (Hpq := ↓ ⇓ (Hpr ↕ Hrq)) (⇓ Hq) ε
@@ -202,22 +204,22 @@ Definition cohFrameSnHyp {n p q r} {ε ω: side} {Hpr: p.+3 <= r.+3}
   frame'.(cohFrame) (Hpr := ↓ Hpr) (Hrq := Hrq) (Hq := Hq) d.
 
 Definition mkCohLayer {n p q r} {ε ω: side} {Hpr: p.+3 <= r.+3}
-  {Hrq: r.+3 <= q.+3} {Hq: q.+3 <= n.+1} {C: Cubical n} {D: mkcsp}
+  {Hrq: r.+3 <= q.+3} {Hq: q.+3 <= n.+1} {C: NType n} {D: mkcsp}
   {Frame: PartialFrame n.+1 p mkcsp mkFramePrev}
   {d: Frame.(frame) (↓ ↓ ↓ (Hpr ↕ Hrq ↕ Hq)) D} (l: mkLayer):
-  let sl := C.(SubLayer') (Hpq := ⇓ (Hpr ↕ Hrq)) ε
-              (mkSubLayer (Hpq := ⇓ Hpr) d l) in
-  let sl' := C.(SubLayer') (Hpq := ⇓ Hpr) ω
-               (mkSubLayer (Hpq := ↓ (Hpr ↕ Hrq)) d l) in
+  let sl := C.(RestrLayer') (Hpq := ⇓ (Hpr ↕ Hrq)) ε
+              (mkRestrLayer (Hpq := ⇓ Hpr) d l) in
+  let sl' := C.(RestrLayer') (Hpq := ⇓ Hpr) ω
+               (mkRestrLayer (Hpq := ↓ (Hpr ↕ Hrq)) d l) in
   rew [C.(Layer'')] cohFrameSnHyp in sl = sl'.
 Proof.
   intros *.
   subst sl sl'; apply functional_extensionality_dep; intros 𝛉; unfold Layer''.
   rewrite <- map_subst_app with
     (P := fun 𝛉 x => C.(FillerPrev).(filler'') (C.(FramePrev).(restrFrame') _ 𝛉 x))
-    (f := C.(SubLayer') _ (mkSubLayer d l))
+    (f := C.(RestrLayer') _ (mkRestrLayer d l))
     (H := cohFrameSnHyp).
-  unfold SubLayer', cohFrameSnHyp, mkSubLayer.
+  unfold RestrLayer', cohFrameSnHyp, mkRestrLayer.
   rewrite <- map_subst with (f := C.(FillerPrev).(restrFiller') (⇓ Hq) ε).
   rewrite <- map_subst with (f := C.(FillerPrev).(restrFiller') (⇓ (Hrq ↕ Hq)) ω).
   rewrite rew_map with
@@ -229,28 +231,28 @@ Proof.
   rewrite rew_map with
     (P := fun x => (C.(FillerPrev).(filler'') x).(Dom))
     (f := fun x => (C.(FramePrev).(restrFrame') (⇓ (Hrq ↕ Hq)) ω x)).
-  rewrite <- (C.(Cube).(cohFiller) (Hrq := ⇓ Hrq) (Hq := ⇓ Hq)).
+  rewrite <- (C.(Filler).(cohFiller) (Hrq := ⇓ Hrq) (Hq := ⇓ Hq)).
   repeat rewrite rew_compose.
   apply rew_swap with (P := fun x => (C.(FillerPrev).(filler'') x).(Dom)).
   rewrite rew_app. now reflexivity. now apply C.(FramePrev).(frame'').
 Qed.
 
 #[local]
-Instance mkCubePrev {n} {C: Cubical n} : PartialFillerPrev n.+1 mkcsp mkFramePrev :=
+Instance mkCubePrev {n} {C: NType n} : PartialFillerPrev n.+1 mkcsp mkFramePrev :=
 {|
-  filler' (p: nat) (Hp: p.+1 <= n.+1) (D: mkcsp) := C.(Cube).(filler) D.2:
+  filler' (p: nat) (Hp: p.+1 <= n.+1) (D: mkcsp) := C.(Filler).(filler) D.2:
     mkFramePrev.(frame') Hp D -> HSet; (* Bug? *)
   filler'' (p: nat) (Hp: p.+2 <= n.+1) (D: mkcsp)
     (d : mkFramePrev.(frame'') Hp D) :=
     C.(FillerPrev).(filler') d;
   restrFiller' (p q: nat) (Hpq: p.+2 <= q.+2) (Hq: q.+2 <= n.+1) (ε: side)
-    (D: mkcsp) (d : _) (b : _) := C.(Cube).(restrFiller) (Hpq := ⇓ Hpq)
+    (D: mkcsp) (d : _) (b : _) := C.(Filler).(restrFiller) (Hpq := ⇓ Hpq)
     (Hq := ⇓ Hq) (E := D.2) b;
 |}.
 
 (* The box at level n.+1 with p = O *)
 #[local]
-Instance mkFrame0 {n} {C: Cubical n}: PartialFrame n.+1 O mkcsp mkFramePrev.
+Instance mkFrame0 {n} {C: NType n}: PartialFrame n.+1 O mkcsp mkFramePrev.
   unshelve esplit.
   * intros; now exact hunit. (* boxSn *)
   * simpl; intros; rewrite C.(eqFrame0). now exact tt. (* restrFrameSn *)
@@ -261,13 +263,13 @@ Defined.
 
 (* The box at level n.+1 with p = S _ *)
 #[local]
-Instance mkFrameSp {n p} {C: Cubical n} {Frame: PartialFrame n.+1 p mkcsp mkFramePrev}:
+Instance mkFrameSp {n p} {C: NType n} {Frame: PartialFrame n.+1 p mkcsp mkFramePrev}:
   PartialFrame n.+1 p.+1 mkcsp mkFramePrev.
   unshelve esplit.
   * intros Hp D; exact {d : Frame.(frame) (↓ Hp) D & mkLayer (d := d)}.
   * simpl; intros * ε * (d, l); invert_le Hpq. (* restrFramep *)
     now exact (rew <- [id] C.(eqFrameSp) in
-      (Frame.(restrFrame) Hq ε d; mkSubLayer d l)).
+      (Frame.(restrFrame) Hq ε d; mkRestrLayer d l)).
   * simpl; intros q r Hpr Hrq Hq ε ω D (d, l). (* cohboxp *)
     invert_le Hpr; invert_le Hrq.
 
@@ -284,17 +286,17 @@ Defined.
 
 (* Finally, we can define mkFrame *)
 #[local]
-Instance mkFrame {n} {C: Cubical n} p: PartialFrame n.+1 p mkcsp mkFramePrev.
+Instance mkFrame {n} {C: NType n} p: PartialFrame n.+1 p mkcsp mkFramePrev.
   induction p.
   + now exact mkFrame0. (* p = O *)
   + now exact (mkFrameSp (Frame := IHp)). (* p = S _ *)
 Defined.
 
-(* For Cube, we take a different strategy. We first define mkfiller,
+(* For Filler, we take a different strategy. We first define mkfiller,
    mkRestrFiller, and lemmas corresponding to their computational properties *)
 (* Fist, for filler *)
 
-Definition mkfiller {n p} {C: Cubical n} {Hp: p <= n.+1} {D: mkcsp}
+Definition mkfiller {n p} {C: NType n} {Hp: p <= n.+1} {D: mkcsp}
   (E: (mkFrame n.+1).(frame) (¹ n.+1) D -> HSet)
   (d: (mkFrame p).(frame) Hp D): HSet.
   revert d; apply le_induction with (Hp := Hp); clear p Hp. (* cubeSn *)
@@ -302,7 +304,7 @@ Definition mkfiller {n p} {C: Cubical n} {Hp: p <= n.+1} {D: mkcsp}
   + intros p Hp IH d; exact {l : mkLayer & IH (d; l)}. (* p = S n *)
 Defined.
 
-Lemma mkfiller_computes {n p} {C: Cubical n} {Hp: p.+1 <= n.+1} {D: mkcsp}
+Lemma mkfiller_computes {n p} {C: NType n} {Hp: p.+1 <= n.+1} {D: mkcsp}
   {E: (mkFrame n.+1).(frame) (¹ n.+1) D -> HSet} {d}:
   mkfiller (Hp := ↓ Hp) E d = {l : mkLayer & mkfiller (Hp := Hp) E (d; l)} :> Type.
 Proof.
@@ -311,14 +313,14 @@ Qed.
 
 (* Now, restrFiller, and the corresponding computational properties. *)
 
-Definition mkRestrFiller {n} {C: Cubical n} {p q} {Hpq: p.+1 <= q.+1}
+Definition mkRestrFiller {n} {C: NType n} {p q} {Hpq: p.+1 <= q.+1}
   {Hq: q.+1 <= n.+1} {ε: side} {D}
   (E: (mkFrame n.+1).(frame) (¹ n.+1) D -> HSet)
   (d: (mkFrame p).(frame) (↓ (Hpq ↕ Hq)) D)
-  (Cube: mkfiller (Hp := ↓ (Hpq ↕ Hq)) E d):
+  (Filler: mkfiller (Hp := ↓ (Hpq ↕ Hq)) E d):
     mkCubePrev.(filler') ((mkFrame p).(restrFrame) Hq ε d).
 Proof.
-  intros *; revert d Cube; simpl. (* subcubeSn *)
+  intros *; revert d Filler; simpl. (* subcubeSn *)
   pattern p, Hpq. (* Bug? Why is this needed? *)
   apply le_induction'.
   + intros d c; rewrite mkfiller_computes in c. destruct c as (l, _).
@@ -327,10 +329,10 @@ Proof.
     rewrite mkfiller_computes in c; destruct c as (l, c).
     change (⇓ (↓ ?Hpq ↕ ?Hq)) with (↓ ⇓ (Hpq ↕ Hq)); rewrite C.(eqFillerSp).
     apply IH in c.
-    now exact (mkSubLayer d l; c).
+    now exact (mkRestrLayer d l; c).
 Defined.
 
-Lemma mkRestrFiller_base_computes {p n} {C: Cubical n} {Hp: p.+1 <= n.+1}
+Lemma mkRestrFiller_base_computes {p n} {C: NType n} {Hp: p.+1 <= n.+1}
   {ε: side} {D E} {d: (mkFrame p).(frame) _ D} {c}:
   mkRestrFiller (Hq := Hp) E d c =
   match (rew [id] mkfiller_computes in c) with
@@ -340,12 +342,12 @@ Proof.
   unfold mkRestrFiller; now rewrite le_induction'_base_computes.
 Qed.
 
-Lemma mkRestrFiller_step_computes {q r n} {C: Cubical n} {Hq: q.+2 <= n.+1}
+Lemma mkRestrFiller_step_computes {q r n} {C: NType n} {Hq: q.+2 <= n.+1}
   {Hrq: r.+2 <= q.+2} {ε: side} {D E} {d: (mkFrame r).(frame) _ D} {c}:
   mkRestrFiller (Hpq := ↓ Hrq) (Hq := Hq) (ε := ε) E d c =
   match (rew [id] mkfiller_computes in c) with
   | (l; c) => rew <- [id] C.(eqFillerSp) in
-    (mkSubLayer d l; mkRestrFiller (Hpq := Hrq) E (d; l) c)
+    (mkRestrLayer d l; mkRestrFiller (Hpq := Hrq) E (d; l) c)
   end.
 Proof.
   unfold mkRestrFiller; now rewrite le_induction'_step_computes.
@@ -355,7 +357,7 @@ Qed.
   on cohFiller *)
 
 (* The base case is easily discharged *)
-Definition mkCohFiller_base {q r n} {ε ω: side} {C: Cubical n} {D: mkcsp}
+Definition mkCohFiller_base {q r n} {ε ω: side} {C: NType n} {D: mkcsp}
   {Hrq: r.+2 <= q.+2} {Hq: q.+2 <= n.+1}
   {E: (mkFrame n.+1).(frame) (¹ n.+1) D -> HSet}
   (d: (mkFrame r).(frame) (↓ ↓ (Hrq ↕ Hq)) D)
@@ -373,19 +375,19 @@ Definition mkCohFiller_base {q r n} {ε ω: side} {C: Cubical n} {D: mkcsp}
 Qed.
 
 (* A small abbreviation *)
-Definition mkCohFiller p {q r n} {ε ω: side} {C: Cubical n} {D: mkcsp}
+Definition mkCohFiller p {q r n} {ε ω: side} {C: NType n} {D: mkcsp}
   (Hpr: p.+2 <= r.+3) {Hrq: r.+3 <= q.+3} {Hq: q.+3 <= n.+1}
   {E: (mkFrame n.+1).(frame) (¹ n.+1) D -> HSet}
   (d: (mkFrame p).(frame) (↓ ↓ (Hpr ↕ Hrq ↕ Hq)) D)
   (c: mkfiller E d) :=
   rew [mkCubePrev.(filler'')] (mkFrame p).(cohFrame) (Hrq := Hrq) d in
-  C.(Cube).(restrFiller) (ε := ε) (Hpq := ⇓ (Hpr ↕ Hrq)) (Hq := ⇓ Hq)
+  C.(Filler).(restrFiller) (ε := ε) (Hpq := ⇓ (Hpr ↕ Hrq)) (Hq := ⇓ Hq)
     (mkRestrFiller (ε := ω) (Hpq := (⇓ Hpr)) (Hq := ↓ (Hrq ↕ Hq)) E d c) =
-  C.(Cube).(restrFiller) (ε := ω) (Hpq := (⇓ Hpr)) (Hq := ⇓ (Hrq ↕ Hq))
+  C.(Filler).(restrFiller) (ε := ω) (Hpq := (⇓ Hpr)) (Hq := ⇓ (Hrq ↕ Hq))
     (mkRestrFiller (ε := ε) (Hpq := ↓ (Hpr ↕ Hrq)) (Hq := Hq) E d c).
 
 (* The step case is discharged as (mkCohLayer; IHP) *)
-Definition mkCohFiller_step {p q r n} {ε ω: side} {C: Cubical n} {D: mkcsp}
+Definition mkCohFiller_step {p q r n} {ε ω: side} {C: NType n} {D: mkcsp}
   {Hpr: p.+3 <= r.+3} {Hrq: r.+3 <= q.+3} {Hq: q.+3 <= n.+1}
   {E: (mkFrame n.+1).(frame) (¹ n.+1) D -> HSet}
   {d: (mkFrame p).(frame) (↓ ↓ (↓ Hpr ↕ Hrq ↕ Hq)) D}
@@ -409,11 +411,11 @@ Definition mkCohFiller_step {p q r n} {ε ω: side} {C: Cubical n} {D: mkcsp}
   (Q := fun x => C.(FillerPrev).(filler') (rew <- [id] C.(eqFrameSp') in x))
   (H := (mkFrame p).(cohFrame) (Hpr := ↓ Hpr) (Hrq := Hrq) (Hq := Hq) (ε := ε)
         (ω := ω) (D := D) d)
-  (u := C.(SubLayer') (Hpq := ⇓ (Hpr ↕ Hrq)) (Hq := ⇓ Hq) (D := D.1) ε
-          (mkSubLayer (Hpq := ⇓ Hpr) (Hq := ↓ (Hrq ↕ Hq)) (C := C) (D := D)
+  (u := C.(RestrLayer') (Hpq := ⇓ (Hpr ↕ Hrq)) (Hq := ⇓ Hq) (D := D.1) ε
+          (mkRestrLayer (Hpq := ⇓ Hpr) (Hq := ↓ (Hrq ↕ Hq)) (C := C) (D := D)
           (Frame := mkFrame p) (ε := ω) d l))
   (v := rew [C.(FillerPrev).(filler')] C.(eqRestrFrameSp) in
-    C.(Cube).(restrFiller) (Hpq := ⇓ (Hpr ↕ Hrq)) (Hq := ⇓ Hq) (ε := ε)
+    C.(Filler).(restrFiller) (Hpq := ⇓ (Hpr ↕ Hrq)) (Hq := ⇓ Hq) (ε := ε)
                        (D := D.1) (E := D.2)
                        (mkRestrFiller (Hpq := ⇓ Hpr) (Hq := ↓ (Hrq ↕ Hq))
                        (D := D) (ε := ω) E (d; l) c'))).
@@ -433,7 +435,7 @@ Qed.
 
 (* Build a PartialFiller n.+1 using what we just defined *)
 #[local]
-Instance mkFiller {n} {C: Cubical n}:
+Instance mkFiller {n} {C: NType n}:
   PartialFiller n.+1 mkcsp mkCubePrev mkFrame.
   unshelve esplit; intros p.
   - intros *; now exact mkfiller.
@@ -446,7 +448,7 @@ Instance mkFiller {n} {C: Cubical n}:
 Defined.
 
 #[local]
-Instance mkCubical0: Cubical 0.
+Instance mkNType0: NType 0.
   unshelve esplit.
   - now exact hunit.
   - unshelve esplit.
@@ -477,15 +479,15 @@ Instance mkCubical0: Cubical 0.
   - intros *; exfalso; clear -Hq; now apply leY_contra in Hq.
 Defined.
 
-(* We are now ready to build a Cubical *)
+(* We are now ready to build a NType *)
 #[local]
-Instance mkCubicalSn {n} {C: Cubical n}: Cubical n.+1.
+Instance mkNTypeSn {n} {C: NType n}: NType n.+1.
   unshelve esplit.
   - (* csp *) now exact mkcsp.
   - (* FramePrev *) now exact mkFramePrev.
   - (* Box *) now exact mkFrame.
   - (* FillerPrev *) now exact mkCubePrev.
-  - (* Cube *) now exact mkFiller.
+  - (* Filler *) now exact mkFiller.
   - (* eqFrame0 *) now intros *.
   - (* eqFrame0' *) intros *; now apply C.(eqFrame0).
   - (* eqFrameSp *) now intros *.
@@ -502,15 +504,15 @@ Instance mkCubicalSn {n} {C: Cubical n}: Cubical n.+1.
     now rewrite eq_ind_r_refl, mkRestrFiller_step_computes, rew_rew'.
 Defined.
 
-Definition CubicalAt: forall n, Cubical n.
+Definition NTypeAt: forall n, NType n.
   induction n.
-  - now exact mkCubical0.
-  - now exact mkCubicalSn.
+  - now exact mkNType0.
+  - now exact mkNTypeSn.
 Defined.
 
-CoInductive CubeUniverse n (X: (CubicalAt n).(csp)): Type@{l'} := cons {
-  this: (CubicalAt n).(Frame).(frame) (¹ n) X -> HSet@{l};
-  next: CubeUniverse n.+1 (X; this);
+CoInductive NTypeUniverse n (X: (NTypeAt n).(csp)): Type@{m'} := cons {
+  this: (NTypeAt n).(Frame).(frame) (¹ n) X -> HSet@{m};
+  next: NTypeUniverse n.+1 (X; this);
 }.
 
-Definition CubeInfinity := CubeUniverse 0 tt.
+Definition CubeInfinity := NTypeUniverse 0 tt.
